[Wstecz](../matematyka.md)

# Na ocenÄ™

### Zadanie 1

a)

$`(1+\cos x)(1-\cos x)=\sin ^2 x, \quad x \in \mathbb{R}`$

$`\mathrm{L}= (1+\cos x)(1-\cos x)=1-\cos ^2 x=1-(1-\sin ^2 x)=1-1+\sin ^2 x=\sin ^2 x=\mathrm{P}`$

f)

$`\cos x+\mathrm{tg}^2 x \cos x=\frac{1}{\cos x}, \quad x \in \mathbb{R} \backslash\{\frac{\pi}{2}+k \pi, \quad k \in \mathbb{Z}\}`$

$`\mathrm{L}= \cos x+\mathrm{tg}^2 x \cos x=\cos x+\frac{\sin ^2 x}{\cos ^2 x} \cdot \cos x=\cos x+\frac{\sin ^2 x}{\cos x}=\frac{\cos ^2 x}{\cos x}+\frac{\sin ^2 x}{\cos x}=\frac{\cos ^2 x+\sin ^2 x}{\cos x}=\frac{1}{\cos x}=\mathrm{P}`$

### Zadanie 2

a)

$`\frac{1}{\sin x \cos x}-\frac{\cos x}{\sin x}=\mathrm{tg} x`$

$`\mathrm{L}= \frac{1}{\sin x \cos x}-\frac{\cos x}{\sin x}=\frac{1}{\sin x \cos x}-\frac{\cos ^2 x}{\sin x \cos x}=\frac{1-\cos ^2 x}{\sin x \cos x}=\frac{\sin ^2 x}{\sin x \cos x}=\frac{\sin x}{\cos x}=\mathrm{tg} x=\mathrm{P}`$

f)

$`\frac{\cos x}{1-\sin x}+\frac{\cos x}{1+\sin x}=\frac{2}{\cos x}`$

$`\mathrm{L}=\frac{\cos x}{1-\sin x}+\frac{\cos x}{1+\sin x}=\frac{\cos x(1+\sin x)}{(1-\sin x)(1+\sin x)}+\frac{\cos x(1-\sin x)}{(1-\sin x)(1+\sin x)}=\frac{\cos x+\cos x \sin x+\cos x-\cos x \sin x}{1-\sin ^2 x}=\frac{2 \cos x}{\cos ^2 x}=\frac{2}{\cos x}=\mathrm{P}`$

### Zadanie 3

a)

$`\frac{1-\sin x}{1+\sin x}-\frac{1+\sin x}{1-\sin x}=\frac{-4 \sin x}{\cos ^2 x}, \quad x \in \mathbb{R} \backslash\{\frac{\pi}{2}+k \pi: k \in \mathbb{Z}\}`$

$`\mathrm{L}=\frac{1-\sin x}{1+\sin x}-\frac{1+\sin x}{1-\sin x}=\frac{(1-\sin x)^2-(1+\sin x)^2}{(1+\sin x)(1-\sin x)}=\frac{(1-\sin x-1-\sin x)(1-\sin x+1+\sin x)}{(1+\sin x)(1-\sin x)}=\frac{(-2 \sin x) \cdot 2}{1-\sin ^2 x}=\quad=\frac{-4 \sin x}{\cos ^2 x}=\mathrm{P}`$

f)

$`\frac{\mathrm{tg} x-\mathrm{ctg} x}{\mathrm{tg} x+\mathrm{ctg} x}=\frac{\mathrm{tg}^2 x-1}{\mathrm{tg}^2 x+1}, \quad x \in \mathbb{R} \backslash\{\frac{k \pi}{2}: k \in \mathbb{Z}\}`$

$`\mathrm{L}=\frac{\mathrm{tg} x-\mathrm{ctg} x}{\mathrm{tg} x+\mathrm{ctg} x}=\frac{\frac{\sin x}{\cos x}-\frac{\cos x}{\sin x}}{\frac{\sin x}{\cos x}+\frac{\cos x}{\sin x}}=\frac{\frac{\sin ^2 x-\cos ^2 x}{\cos x \sin x}}{\frac{\sin ^2 x+\cos ^2 x}{\cos x \sin x}}=\frac{\sin ^2 x-\cos ^2 x}{\cos x \sin x} \cdot \cos x \sin x=\sin ^2 x-\cos ^2`$

$`\mathrm{P}=\frac{\mathrm{tg}^2 x-1}{\mathrm{tg}^2 x+1}=\frac{\frac{\sin ^2 x}{\cos ^2 x}-1}{\frac{1}{\cos ^2 x}}=\frac{\sin ^2 x-\cos ^2 x}{\cos ^2 x} \cdot \cos ^2 x=\sin ^2 x-\cos ^2 x=\mathrm{L}`$

### Zadanie 4

a)

$`\cos x=-\frac{1}{4} \quad$ i $\quad x \in(\frac{\pi}{2} ; \pi)`$

$`\sin ^2 x+\cos ^2 x=1`$

$`\cos x=-\frac{1}{4}\sin ^2 x+(-\frac{1}{4})^2=1`$

$`\sin ^2 x+\frac{1}{16}=1`$

$`-\frac{1}{16}\sin ^2 x=1-\frac{1}{16}`$

$`\sin ^2 x=\frac{15}{16}`$

$`\sin x=\frac{\sqrt{15}}{4}`$

$`\mathrm{tg} x=\frac{\sin x}{\cos x}=\frac{\frac{\sqrt{15}}{4}}{-\frac{1}{4}}=\frac{\sqrt{15}}{4} \cdot(-4)=-\sqrt{15}\mathrm{ctg} x=\frac{1}{\mathrm{tg} x}=-\frac{1}{\sqrt{15}}=-\frac{\sqrt{15}}{15}`$

d)

$`\sin x=-\frac{\sqrt{10}}{10} \quad \text { i } \quad x \in(\frac{3}{2} \pi ; 2 \pi)`$

$`x \in(\frac{3}{2} \pi ; 2 \pi)`$

$`\cos x>0, \quad \mathrm{tg} x<0, \quad \mathrm{ctg} x<0`$

$`\sin ^2 x+\cos ^2 x=1`$

$`\sin x=-\frac{\sqrt{10}}{10} (-\frac{\sqrt{10}}{10})^2+\cos ^2 x=1`$

$`\frac{10}{100}+\cos ^2 x=1`$

$`\cos ^2 x=1-\frac{10}{100}`$

$`\cos ^2 x=\frac{90}{100}`$

$`x=\frac{\sqrt{90}}{10}=\frac{3 \sqrt{10}}{10}`$

$`\mathrm{tg} x=\frac{\sin x}{\cos x}=\frac{-\frac{\sqrt{10}}{10}}{\frac{3 \sqrt{10}}{10}}=-\frac{\sqrt{10}}{10} \cdot \frac{10}{3 \sqrt{10}}=-\frac{1}{3}\mathrm{ctg} x=\frac{1}{\mathrm{tg} x}=-3`$

### Zadanie 5

a)

$`\sin x=\frac{1}{3}`$

$`\sin ^2 x+\cos ^2 x=1`$

$`(\frac{1}{3})^2+\cos ^2 x=1`$

$`\frac{1}{9}+\cos ^2 x=1`$

$`\cos ^2 x=\frac{8}{9}`$

$`\cos x=\frac{2 \sqrt{2}}{3} \quad \vee \quad \cos x=-\frac{2 \sqrt{2}}{3}`$

$`\mathrm{tg} x=\frac{\sin x}{\cos x}`$

$`\mathrm{tg} x=\frac{\frac{1}{3}}{\frac{2 \sqrt{2}}{3}}=\frac{1}{3} \cdot \frac{3}{2 \sqrt{2}}=\frac{1}{2 \sqrt{2}}=\frac{\sqrt{2}}{4} \quad \vee \quad \mathrm{tg} x=\frac{\frac{1}{3}}{-\frac{2 \sqrt{2}}{3}}=\frac{1}{3} \cdot\left(-\frac{3}{2 \sqrt{2}}\right)=-\frac{1}{2 \sqrt{2}}=-\frac{\sqrt{2}}{4}`$

$`\mathrm{ctg} x=2 \sqrt{2} \quad \vee \quad \mathrm{ctg} x=-2 \sqrt{2}`$

$$
\left\{\begin{array} { l }
{ \cos x = \frac { 2 \sqrt { 2 } } { 3 } } \\
{ \operatorname { t g } x = \frac { \sqrt { 2 } } { 4 } } \\
{ \mathrm{ctg} x = 2 \sqrt { 2 } }
\end{array} \quad \vee \quad \left\{\begin{array}{l}
\cos x=-\frac{2 \sqrt{2}}{3} \\
\mathrm{tg} x=-\frac{\sqrt{2}}{4} \\
\mathrm{ctg} x=-2 \sqrt{2}
\end{array}\right.\right.
$$

h)

$`\cos x=\frac{\sqrt{21}}{5}`$

$`\sin ^2 x+\cos ^2 x=1`$

$`\sin ^2 x^2+\left(\frac{\sqrt{21}}{5}\right)^2=1`$

$`\sin ^2 x+\frac{21}{25}=1`$

$`\sin ^2 x=\frac{4}{25}`$

$`\sin x=\frac{2}{5} \quad \vee \quad \sin x=-\frac{2}{5}`$

$`\mathrm{tg} x=\frac{\sin x}{\cos x}`$

$`\mathrm{tg} x=\frac{\frac{2}{5}}{\frac{\sqrt{21}}{5}}=\frac{2}{5} \cdot\left(\frac{5}{\sqrt{21}}\right)=\frac{2}{\sqrt{21}}=\frac{2 \sqrt{21}}{21} \quad \vee \quad \mathrm{tg} x =\frac{-\frac{2}{5}}{\frac{\sqrt{21}}{5}}=-\frac{2}{5} \cdot\left(\frac{5}{\sqrt{21}}\right)=-\frac{2}{\sqrt{21}}=-\frac{2 \sqrt{21}}{21} \mathrm{ctg} x=\frac{\sqrt{21}}{2} \vee \quad \mathrm{ctg} x=-\frac{\sqrt{21}}{2}`$

$$
\left\{\begin{array} { l }
{ \sin x = \frac { 2 } { 5 } } \\
{ \operatorname { t g } x = \frac { 2 \sqrt { 2 1 } } { 2 1 } } \\
{ \mathrm{ctg} x = \frac { \sqrt { 2 1 } } { 2 } }
\end{array} \quad \vee \quad \left\{\begin{array}{l}
\sin x=-\frac{2}{5} \\
\mathrm{tg} x=-\frac{2 \sqrt{21}}{21} \\
\mathrm{ctg} x=-\frac{\sqrt{21}}{2}
\end{array}\right.\right.
$$

### Zadanie 6

$`\mathrm{tg} x=-\frac{1}{2} \quad \text { i } \quad x \in\left(\frac{\pi}{2} ; \pi\right)`$

$`x \in\left(\frac{\pi}{2} ; \pi\right)`$

$`\sin x>0, \quad \cos x<0, \quad \mathrm{ctg} x<0`$

$`\mathrm{tg} x=\frac{\sin x}{\cos x}`$

$`-\frac{1}{2}=\frac{\sin x}{\cos x}`$

$`\sin x=-\frac{1}{2} \cos x`$

$`\sin ^2 x+\cos ^2 x=1, \sin x=-\frac{1}{2} \cos x`$

$`\left(-\frac{1}{2} \cos x\right)^2+\cos ^2 x=1`$

$`\frac{1}{4} \cos ^2 x+\cos ^2 x=1`$

$`\frac{5}{4} \cos ^2 x=1`$

$`\cos ^2 x=\frac{4}{5}`$

$`\cos x=\frac{2}{\sqrt{5}}=-\frac{2 \sqrt{5}}{5}`$

$`\sin x=-\frac{1}{2} \cos x=-\frac{1}{2} \cdot\left(-\frac{2 \sqrt{5}}{5}\right)=\frac{\sqrt{5}}{5}`$

$`\mathrm{ctg} x=-2`$

d)

$`\mathrm{ctg} x=\frac{2}{3} \mathrm{i} x \in\left(\pi ; \frac{3}{2} \pi\right)`$

$`x \in\left(\pi ; \frac{3}{2} \pi\right)`$

$`\mathrm{ctg} x=\frac{\cos x}{\sin x}`$

$`\frac{2}{3}=\frac{\cos x}{\sin x}`$

$`\sin x=\frac{3}{2} \cos x`$

$`\sin x<0, \quad \cos x<0, \quad \mathrm{tg} x>0`$

$`\sin ^2 x+\cos ^2 x=1, \sin x=\frac{3}{2} \cos x`$

$`\left(\frac{3}{2} \cos x\right)^2+\cos ^2 x=1`$

$`\frac{9}{4} \cos ^2 x+\cos ^2 x=1`$

$`\frac{13}{4} \cos ^2 x=1`$

$`\cos ^2 x=\frac{4}{13}`$

$`\cos x=-\frac{2}{\sqrt{13}}=-\frac{2 \sqrt{13}}{13}`$

$`\sin x=\frac{3}{2} \cos x=\frac{3}{2} \cdot\left(-\frac{2 \sqrt{13}}{13}\right)=-\frac{3 \sqrt{13}}{13}`$

$`\mathrm{tg} x=\frac{3}{2}`$

### Zadanie 7

a)

$`\mathrm{tg} x=\frac{3}{4}`$

$`\mathrm{tg} x=\frac{\sin x}{\cos x}`$

$`\frac{3}{4}=\frac{\sin x}{\cos x}`$

$`\sin x=\frac{3}{4} \cos x`$

$`\sin ^2 x+\cos ^2 x=1`$

$`\left(\frac{3}{4} \cos x\right)^2+\cos ^2 x=1`$

$`\frac{9}{16} \cos ^2 x+\cos ^2 x=1`$

$`\frac{25}{16} \cos ^2 x=1`$

$`\cos ^2 x=\frac{16}{25}`$

$`\cos x=\frac{4}{5} \quad \vee \quad \cos x=-\frac{4}{5}`$

$`\sin x=\frac{3}{4} \cdot \cos x`$

$`\sin x=\frac{3}{4} \cdot \frac{4}{5} \vee \sin x=\frac{3}{4} \cdot\left(-\frac{4}{5}\right)`$

$`\sin x=\frac{3}{5} \vee \sin x=-\frac{3}{5}`$

$`\mathrm{ctg} x=\frac{4}{3}`$

$$
\left\{\begin{array} { l }
{ \cos x = \frac { 4 } { 5 } } \\
{ \sin x = \frac { 3 } { 5 } } \\
{ \mathrm{ctg} x = \frac { 4 } { 3 } }
\end{array} \quad \vee \quad \left\{\begin{array}{l}
\cos x=-\frac{4}{5} \\
\sin x=-\frac{3}{5} \\
\mathrm{ctg} x=\frac{4}{3}
\end{array}\right.\right.
$$

d)

$`\mathrm{tg} x=\frac{1}{2}`$

$`\mathrm{tg} x=\frac{\sin x}{\cos x}`$

$`\frac{1}{2}=\frac{\sin x}{\cos x}`$

$`\sin x=\frac{1}{2} \cos x`$

$`\sin ^2 x+\cos ^2 x=1`$

$`\left(\frac{1}{2} \cos x\right)^2+\cos ^2 x=1`$

$`\frac{1}{4} \cos ^2 x+\cos ^2 x=1`$

$`\frac{5}{4} \cos ^2 x=1`$

$`\cos ^2 x=\frac{4}{5}`$

$`\cos x=\frac{2}{\sqrt{5}}=\frac{2 \sqrt{5}}{5} \quad \vee \quad \cos x=-\frac{2}{\sqrt{5}}=-\frac{2 \sqrt{5}}{5}`$

$`\sin x=\frac{1}{2} \cdot \cos x`$

$`\sin x=\frac{1}{2} \cdot \frac{2 \sqrt{5}}{5} \quad \vee \quad \sin x=\frac{1}{2} \cdot\left(-\frac{2 \sqrt{5}}{5}\right)`$

$`\sin x=\frac{\sqrt{5}}{5} \quad \vee \quad \sin x=-\frac{\sqrt{5}}{5}`$

$`\mathrm{ctg} x=2`$

$$
\left\{\begin{array} { l }
{ \cos x = \frac { 2 \sqrt { 5 } } { 5 } } \\
{ \sin x = \frac { \sqrt { 5 } } { 5 } } \\
{ \mathrm{ctg} x = 2 }
\end{array} \quad \vee \quad \left\{\begin{array}{l}
\cos x=-\frac{2 \sqrt{5}}{\sqrt{5}} \\
\sin x=-\frac{\sqrt{5}}{5} \\
\mathrm{ctg} x=2
\end{array}\right.\right.
$$

---

### Zadanie 3

a) $`\sin 120=\sin (180-60)=\sin 60=\frac{\sqrt{3}}{2}`$

b) $`\sin 135=\sin (180-45)=\sin 45=\frac{\sqrt{2}}{2}`$

c) $`\cos 330=\cos (360-30)=\cos 30=\frac{\sqrt{3}}{2}`$

d) $`\cos 495=\cos (360+135)=\cos 135=\cos (180-45)=-\cos 45=-\frac{\sqrt{2}}{2}`$

e) $`\cos 840=\cos (2 \cdot 360+120)=\cos 120=\cos (180-60)=-\cos 60=-\frac{1}{2}`$

f) $`\sin 660=\sin (360+300)=\sin 300=\sin (360-60)=-\sin 60=-\frac{\sqrt{3}}{2}`$

g) $`\mathrm{tg} 510=\mathrm{tg}(360+150)=\mathrm{tg} 150=\mathrm{tg}(180-30)=-t g 30=-\frac{\sqrt{3}}{3}`$

h) $`\mathrm{tg} 570=\mathrm{tg}(360+210)=\mathrm{tg} 210=\mathrm{tg}(180+30)=\mathrm{tg} 30=\frac{\sqrt{3}}{3}`$

i) $`\mathrm{tg} 1035=\mathrm{tg}(2 \cdot 360+315)=\mathrm{tg} 315=\mathrm{tg}(360-45)=-\mathrm{tg} 45=-1`$

j) $`\sin (-870)=-\sin (870)=-\sin (2 \cdot 360+150)=-\sin 150=-\sin (180-30)=-\sin 30=-\frac{1}{2}`$

k) $`\mathrm{tg}(-330)=-\mathrm{tg} 330=-\mathrm{tg}(360-30)=-(-\mathrm{tg} 30)=\mathrm{tg} 30=\frac{\sqrt{3}}{3}`$

l) $`\mathrm{ctg}(-\alpha)=-\mathrm{ctg} \alpha`$

$`\mathrm{ctg}(-750)=-\mathrm{ctg} 750=-\mathrm{ctg}(2 \cdot 360+30)=-\mathrm{ctg} 30=-\sqrt{3}`$

### Zadanie 4

e) $`\sin \left(-468^{\circ}\right)=-\sin 468^{\circ}=-\sin \left(450^{\circ}+18^{\circ}\right)=-\sin \left(90^{\circ}+18^{\circ}\right)=-\cos 18^{\circ}=-\frac{\sqrt{10+2 \sqrt{5}}}{4}`$

f) $`\cos \left(-864^{\circ}\right)=\cos 864^{\circ}=\cos \left(810^{\circ}+54^{\circ}\right)=\cos \left(90^{\circ}+54^{\circ}\right)=-\sin 54^{\circ}=-\frac{\sqrt{5}+1}{4}`$
