[Wstecz](../matematyka.md)

# Potęga o wykładniku rzeczywistym

$`\sqrt3 \approx 1,7321`$

$`5^{\sqrt3} \approx 5^{1,7321} \approx 16,2437`$

Dla dowolnych liczb $`a, b \in \R`$ i dowolnych $`x, y \in \R`$ prawdziwe są wzory:

1. $`a^x \cdot a^y = a^{x+y}`$
2. $`\frac{a^x}{a^y} = a^{x-y}`$
3. $`(a^x)^y = a^{x \cdot y}`$
4. $`a^x \cdot b^x = ab^x`$

### Ćwiczenie 4/286

b) $`(3^{\sqrt2})^{2\sqrt2} = 3^{\sqrt2 \cdot 2 \sqrt2} = 3^4 = 81`$

d) $`(2^{\sqrt7 - \sqrt2})^{\sqrt7 + \sqrt2} = 2^{(\sqrt7 - \sqrt2) \cdot (\sqrt7 + \sqrt2)} = 2^{7 - 2} = 2^5 = 32`$

f) $`9^{\sqrt5} \cdot 3^{1 - 2 \sqrt5} = 3^{2 \sqrt5} \cdot 3^{1-2 \sqrt5} = 3^1 = 3`$

h) $`\frac{6^{\sqrt3 + 1} \cdot 2^{\sqrt{-3}}}{3^{\sqrt3}} = \frac{6{\sqrt3} \cdot 6 \cdot 2^{\sqrt{-3}}}{3^{\sqrt3}} = \frac{2^{\sqrt3} \cdot 3^{\sqrt3} \cdot 2^{\sqrt{-3}}}{3^{\sqrt3}} = 1 \cdot 6 = 6`$

### Zadanie 1/287

a) $`3^4 \cdot 3^{1-\sqrt{2}}=3^{4+1-\sqrt{2}}=3^{5-\sqrt{2}}`$

b) $`3^3: 3^{2-\sqrt{2}}=3^{3-(2-\sqrt{2})}=3^{3-2+\sqrt{2}}=3^{1+\sqrt{2}}`$

c) $`(3^{\sqrt{7}-\sqrt{3}})^{\sqrt{7}+\sqrt{3}}=3^{(\sqrt{7}-\sqrt{3})(\sqrt{7}+\sqrt{3})}=3^{\sqrt{7^2-\sqrt{3}}}=3^{7-3}=3^4`$

d) $`(3^{\sqrt{3}})^{1-\sqrt{3}}=3^{\sqrt{3}(1-\sqrt{3})}=3^{\sqrt{3}-3}`$

e) $`6^{\sqrt{7}}: 2^{\sqrt{7}}=(6: 2)^{\sqrt{7}}=3^{\sqrt{7}}`$

f) $`(\sqrt{3})^\pi \cdot(\sqrt{3})^\pi=\sqrt{3}^{\pi+\pi}=\sqrt{3}^{2 \pi}=(\sqrt{3}^2)^\pi=3^\pi`$

### Zadanie 2/287

a) $`6^{1-\sqrt{2}} \cdot 6^{\sqrt{2}+1}=6^{1-\sqrt{2}+\sqrt{2}+1}=6^2=36`$

b) $`5^{\pi+3}: 5^\pi=5^{\pi+3-\pi}=5^3=125`$

c) $`(\frac{3}{5})^{\sqrt{6}-1} \cdot(\frac{5}{3})^{\sqrt{6}+2}=(\frac{3}{5})^{\sqrt{6}-1} \cdot((\frac{3}{5})^{-1})^{\sqrt{6}+2}=(\frac{3}{5})^{\sqrt{6}-1} \cdot(\frac{3}{5})^{-\sqrt{6}-2}=(\frac{3}{5})^{\sqrt{6}-1-\sqrt{6}-2}=(\frac{3}{5})^{-3}=(\frac{5}{3})^3=\frac{125}{27}`$

d) $`2^{3 \sqrt{5}} \cdot 8^{-\sqrt{5}}=2^{3 \sqrt{5}} \cdot(2^3)^{-\sqrt{5}}=2^{3 \sqrt{5}} \cdot 2^{-3 \sqrt{5}}=2^{3 \sqrt{5}+(-3 \sqrt{5})}=2^0=1`$

e) $`4^{\sqrt{3}}: 2^{2 \sqrt{3}}=(2^2)^{\sqrt{3}}: 2^{2 \sqrt{3}}=2^{2 \sqrt{3}}: 2^{2 \sqrt{3}}=2^{2 \sqrt{3}-2 \sqrt{3}}=2^0=1`$

f) $`\frac{7^{\frac{5}{6}}}{7^{\frac{1}{3}} \sqrt{7}} \cdot \frac{7^{\sqrt{5}+5}}{7^{\sqrt{5}+2}}=\frac{7^{\frac{5}{6}}}{7^{\frac{1}{3}} \cdot 7^{\frac{1}{2}}} \cdot 7^{\sqrt{5}+5-(\sqrt{5}+2)}=\frac{7^{\frac{5}{8}}}{7^{\frac{1}{3}+\frac{1}{2}}} \cdot 7^{\sqrt{5}+5-\sqrt{5}-2}=\frac{7^{\frac{5}{6}}}{7^{\frac{2}{8}+\frac{3}{8}}} \cdot 7^3=\frac{7^{\frac{5}{6}}}{7^{\frac{5}{8}}} \cdot 7^3=343`$

g) $`6^{\sqrt{3}} \cdot 3^{1-\sqrt{3}} \cdot 2^{-\sqrt{3}}=2^{\sqrt{3}} \cdot 3^{\sqrt{3}} \cdot 3^{1-\sqrt{3}} \cdot 2^{-\sqrt{3}}=2^{\sqrt{3}-\sqrt{3}} \cdot 3^{\sqrt{3}+1-\sqrt{3}}=2^0 \cdot 3^1=1 \cdot 3=3`$

h) $`4^{\pi+3} \cdot 3^\pi: 12^\pi=\frac{4^\pi \cdot 4^3 \cdot 3^\pi}{12^\pi}=\frac{(4 \cdot 3)^\pi \cdot 4^3}{12^\pi}=\frac{12^\pi \cdot 4^3}{12^\pi}=4^3=64`$

i) $`\frac{6^{\frac{2}{3}} \cdot 6^{\frac{3}{2}}}{6^{\frac{1}{6}}} \cdot(6^{\sqrt{5}-2})^{\sqrt{5}+2}=\frac{6^{\frac{2}{3}+\frac{2}{2}}}{6^{\frac{1}{6}}} \cdot 6^{\sqrt{5}-2}(\sqrt{5}+2)=\frac{6^{\frac{4}{6}+\frac{8}{6}}}{6^{\frac{1}{6}}} \cdot 6^{5-4}=\frac{6^{\frac{13}{6}}}{6^{\frac{1}{8}}} \cdot 6^1=6^{\frac{13}{6}-\frac{1}{6}} \cdot 6^1=6^2 \cdot 6^1=36 \cdot 6=216`$

### Zadanie 3/287

a) $`2^{\sqrt{7}-2} \cdot 4^3=2^{\sqrt{7}-2} \cdot(2^2)^3=2^{\sqrt{7}-2} \cdot 2^6=2^{\sqrt{7}-2+6}=2^{\sqrt{7}+4}`$

b) $`2^{\sqrt{3}} \cdot \sqrt{2}=2^{\sqrt{3}} \cdot 2^{\frac{1}{2}}=2^{\sqrt{3}+\frac{1}{2}}`$

c) $`9^{\frac{\sqrt{5}}{2}} \cdot 27^{-1}=(3^2)^{\frac{\sqrt{5}}{2}} \cdot(3^3)^{-1}=3^{2 \cdot \frac{\sqrt{5}}{2}} \cdot 3^{-3}=3^{\sqrt{5}} \cdot 3^{-3}=3^{\sqrt{5}-3}`$

d) $`27 \cdot(3^{-\sqrt{3}})^2=3^3 \cdot 3^{-2 \sqrt{3}}=3^{3-2 \sqrt{3}}`$

e) $`\frac{1}{3} \cdot 9^{\pi+\frac{1}{2}}: 81^{2 \pi}=\frac{1}{3} \cdot 9^{\frac{1}{2}} \cdot 9^\pi:(9^2)^{2 \pi}=\frac{1}{3} \cdot 3 \cdot 9^\pi: 9^{4 \pi}=9^{\pi-4 \pi}=9^{-3 \pi}=(3^2)^{-3 \pi}=3^{-6 \pi}`$

f) $`7^{-2 \sqrt{2}}: 49^{\pi+\sqrt{2}}=7^{-2 \sqrt{2}}:(7^2)^{\pi+\sqrt{2}}=7^{-2 \sqrt{2}}: 7^{2 \pi+2 \sqrt{2}}=7^{-2 \sqrt{2}-2 \pi-2 \sqrt{2}}=7^{-4 \sqrt{2}-2 \pi}`$
