[Wstecz](../matematyka.md)

# Przekształcanie podstawy logarytmu

$`\log_bx=\frac{\log_ax}{\log_ab}`$

$`\log_410=\frac{\log_210}{\log_24}=\frac{\log_210}{2}=0,5\log_210=\log_2\sqrt{10}`$

$`\log_ab\cdot\log_bx=\log_ax`$

$`\log_23\cdot\log_34\cdot\log_45\cdot\log_56\cdot\log_67\cdot\log_78=\log_28=3`$

$`\log_ab=\frac{1}{\log_ba}`$

$`\log_27=\frac{\log_27}{\log_72}=\frac{1}{\log_72}`$

<hr>

### Zad 1/315

**a.** $`\log_{16}3=\frac{\log_23}{\log_216}=\frac{\log_23}{4}=0,25\log_23=\log_2\sqrt[4]{3}`$

**c.** $`\log_{\sqrt2}11=\frac{\log_211}{\log_2\sqrt2}=\frac{\log_211}{0,5}=2\log_211=\log_2121`$

**e.** $`\log_46+\log_86=\frac{\log_26}{\log_24}+\frac{\log_26}{\log_28}=\frac{\log_26}{2}+\frac{\log_26}{3}=0,5\log_26+\frac{1}{3}\log_26=\frac{5}{6}\log_26=\log_26^{\frac{5}{6}}`$

### Zad 2/315

**b.**

$`\log_{\frac12}9+\log_49=\log_2\frac{1}{3}`$

$`L=\log_{\frac12}9+\log_49`=\frac{\log_29}{\log_2\frac12}+\frac{\log_29}{\log_24}=\frac{\log_29}{-1}+\frac{\log_29}{2}=-1\log_29+\frac12\log_29=-\frac12\log_29=\log_29^{-\frac12}=\log_2\frac{1}{3}`$

$`L=P`$

### Zad 8/317

$`\log_da=0,5`$

**a.**

$`a>0, a\not=1, b>0, b\not=1, c>0, c\not=1, d>0`$

$`\log_ab\cdot\log_bc\cdot\log_cd=\log_ad=\frac{1}{\log_da}=\frac{1}{0,5}=2`$

## Praca Własna

### Zad 1/315

**b.** $`\log_{0,5} 7=\frac{\log_2 7}{\log_2 0,5}=\frac{\log_2 7}{\log_2(\frac{1}{2})}=\frac{\log_2 7}{-1}=-\log_2 7=\log_2 7^{-1}=\log_2(\frac{1}{7})`$

**d.** $`\log_{\frac{1}{8}} 9=\frac{\log_2 9}{\log_2(\frac{1}{8})}=\frac{\log_2 9}{-3}=-\frac{1}{3} \log_2 9=\log_2 9^{-\frac{1}{3}}=\log_2 \sqrt[3]{\frac{1}{9}}`$

**f.** $`\log_{\frac{1}{2}} 3+\log_{\frac{1}{4}} 3+\log_{0,125} 3=\frac{\log_2 3}{\log_2(\frac{1}{2})}+\frac{\log_2 3}{\log_2(\frac{1}{4})}+\frac{\log_2 3}{\log_2 0,125}=\frac{\log_2 3}{-1}+\frac{\log_2 3}{-2}+\frac{\log_2 3}{\log_2(\frac{1}{8})}=-\log_2 3-\frac{1}{2} \log_2 3+\frac{\log_2 3}{-3}=\log_2 3^{-1}+\log_2 3^{-\frac{1}{2}}-\frac{1}{3} \log_2 3=\log_2 3^{-1}+\log_2 3^{-\frac{1}{2}}+\log_2 3^{-\frac{1}{3}}=\log_2(3^{-1} \cdot 3^{-\frac{1}{2}} \cdot 3^{-\frac{1}{3}})=\log_2 3^{-1-\frac{1}{2}-\frac{1}{3}}=\log_2 3^{-\frac{11}{6}}`$

### Zad 2/315

**a.**

$\log _2 25+\log _4 25=\log _2 125$

$`L=\log _2 25+\frac{\log _2 25}{\log _2 4}=\log _2 25+\frac{\log _2 25}{2}=\log _2 25+\frac{1}{2} \log _2 25=\frac{3}{2} \log _2 25=\log _2 25^{\frac{3}{2}}=\log _2 \sqrt{25^3}=\log _2 125`$

$`P=\log _2 125`$

$`L=P`$

**b.**

$\log _{0,1} 4+\log _{0,01} 16=\log \frac{1}{16}$

$`L=\frac{\log 4}{\log 0,1}+\frac{\log 16}{\log 0,01}=\frac{\log 4}{-1}+\frac{\log 16}{-2}=-\log 4-\frac{1}{2} \log 16=-\log 4-\log 16^{\frac{1}{2}}=-\log 4-\log 4=-2 \log 4=\log 4^{-2}=\log \frac{1}{16}`$

$`P=\log \frac{1}{16}`$

$`L=P`$

**c.**

$\log _3 4+\log _9 4=\log _{\frac{1}{3}} 0,125$

$`L=\frac{\log _{\frac{1}{3}} 4}{\log _{\frac{1}{3}} 3}+\frac{\log _{\frac{1}{3}} 4}{\log _{\frac{1}{3}} 9}=\frac{\log _{\frac{1}{3}} 4}{-1}+\frac{\log _{\frac{1}{3}} 4}{-2}=-\log _{\frac{1}{3}} 4-\frac{1}{2} \log _{\frac{1}{3}} 4=-\frac{3}{2} \log _{\frac{1}{3}} 4=\log _{\frac{1}{3}} 4^{-\frac{3}{2}}=\log _{\frac{1}{3}} \sqrt{(\frac{1}{4})^3}=\log _{\frac{1}{3}} \frac{1}{8}`$

$`P=\log _{\frac{1}{3}} 0,125=\log _{\frac{1}{3}} \frac{125}{1000}=\log _{\frac{1}{3}} \frac{1}{8}`$

$`L=P`$

### Zad 1/307

**a.**

$`3=\log _a 27`$

$`a^3=27`$

$`a=\sqrt[3]{27}`$

$`a=3`$

**d.**

$`4=\log _a 4`$

$`a^4=4`$

$`a=\sqrt[4]{4}`$

$`a=4^{\frac{1}{4}}`$

$`a=(2^2)^{\frac{1}{4}}`$

$`a=2^{\frac{1}{2}}`$

$`a=\sqrt{2}`$

### Zad 2/307

**a.**

$`D_f=(0,1)`$

$`Z W_f=(-\infty, 0)`$

**d.**

$`D_f=\langle\frac{\sqrt{2}}{2}, 1024\rangle`$

$`y=\log _2(\frac{\sqrt{2}}{2})`$

$`2^y=\frac{\sqrt{2}}{2}`$

$`2^y=\frac{2^{\frac{1}{2}}}{2^1}`$

$`2^y=2^{\frac{1}{2}-1}`$

$`2^y=2^{-\frac{1}{2}}`$

$`y=-\frac{1}{2}`$

$`y=\log _2 1024`$

$`2^y=1024`$

$`2^y=2^{10}`$

$`y=10`$

$`Z W_f=\langle-\frac{1}{2}, 10\rangle`$
