[Wstecz](../matematyka.md)

# Tożsamości trygonometryczne

$`\sin^2x+\cos^2x=1`$

$`\tg x=\frac{\sin x}{\cos x}`$

$`\ctg x=\frac{\cos x}{\sin x}`$

$`\ctg x=\frac{1}{\tg x}`$

$`\tg x=\frac{1}{\ctg x}`$

---

### Ćwiczenie 2/49

$`(1-\tg x)(1+\ctg x)=\ctg x-\tg x \text{ dla } x \in \R \backslash\{\frac{k \pi}{2}: k \in \Z\}`$

$`L = (1-\tg x)(1+\ctg x) = 1 + \ctg x - \tg x - \tg x \cdot \ctg x = 1 + \ctg x - \tg x - \tg x \cdot \frac{1}{\tg x} = 1 + \ctg x - \tg x - 1 = \ctg x - \tg x`$

$`L=P`$

